theories/L6_PCPS/uncurry_proto.v
@@ -16,28 +16,6 @@ Require L6.cps.
 Set Universe Polymorphism.
 Unset Strict Unquote Universe Mode.
 
-(** * Auxiliary data used by the rewriter *)
-
-(* true if in cps mode *)
-Definition R_misc : Set := bool.
-
-(* pair of 
-   1 - max number of arguments 
-   2 - encoding of inlining decision for beta-contraction phase *)
-Definition St : Set := (nat * (cps.PM nat))%type.
-(* 0 -> Do not inline, 1 -> uncurried function, 2 -> continuation of uncurried function *)
-
-(* Maps (arity+1) to the right fun_tag *)
-Definition arity_map : Set := cps.PM fun_tag.
-Definition local_map : Set := cps.PM bool.
- 
-(* The state for this includes 
-   1 - a boolean for tracking whether or not a reduction happens
-   2 - Map recording the (new) fun_tag associated to each arity
-   3 - local map from var to if function has already been uncurried
-   4 - Map for uncurried functions for a version of inlining *)
-Definition S_misc : Set := (bool * arity_map * local_map * St * comp_data). 
-
 (** * Uncurrying as a guarded rewrite rule *)
 
 (* Hack: the pretty-printer uses cdata to associate strings with freshly generated names.
@@ -57,119 +35,27 @@ Definition set_name old_var new_var suff cdata :=
 Definition set_names_lst olds news suff cdata :=
   fold_right (fun '(old, new) cdata => set_name old new suff cdata) cdata (combine olds news).
 
-Inductive uncurry_step : exp -> exp -> Prop :=
-(* Uncurrying for CPS *)
-| uncurry_cps :
-  forall (C : frames_t exp_univ_list_fundef exp_univ_exp)
-    (f f1 : var) (ft ft1 : fun_tag) (k k' : var) (kt : fun_tag) (fv fv1 : list var)
-    (g g' : var) (gt : fun_tag) (gv gv1 : list var) (ge : exp) (fds : list fundef)
-    (lhs rhs : list fundef) (s : Ensemble cps.var) (next_x : cps.var)
-    (fp_numargs : nat) (ms : S_misc),
-  (* Non-linear LHS constraints *)
-  k = k' /\
-  g = g' /\
-  (* Guards: *)
-  (* (1) g can't be recursive or invoke k *)
-  ~ ![g] \in used_vars ![ge] /\
-  ~ ![k] \in used_vars ![ge] /\
-  (* (2) gv1, fv1, f1 must be fresh and contain no duplicates *)
-  lhs = Ffun f ft (k :: fv) (Efun [Ffun g gt gv ge] (Eapp k' kt [g'])) :: fds /\
-  rhs = Ffun f ft (k :: fv1) (Efun [Ffun g gt gv1 (Eapp f1 ft1 (gv1 ++ fv1))] (Eapp k kt [g]))
-        :: Ffun f1 ft1 (gv ++ fv) ge :: fds /\
-  s = used_vars (exp_of_proto (C ⟦ lhs ⟧)) /\
-  fresh_copies s gv1 /\ length gv1 = length gv /\
-  fresh_copies (s :|: FromList ![gv1]) fv1 /\ length fv1 = length fv /\
-  ~ ![f1] \in (s :|: FromList ![gv1] :|: FromList ![fv1]) /\
-  (* (3) next_x must be a fresh variable *)
-  fresher_than next_x (s :|: FromList ![gv1] :|: FromList ![fv1] :|: [set ![f1]]) /\
-  (* (4) misc. let bindings (needed for computation of new ms) *)
-  fp_numargs = length fv + length gv /\ ms = ms ->
-  (* 'Irrelevant' guard *)
-  When (fun (is_cps : R_misc) (s : S_misc) =>
-    is_cps &&
-    let '(b, aenv, lm, s, cdata) := s in
-    (* g must not have been already uncurried by an earlier pass *)
-    negb match M.get ![g] lm with
-    | Some true => true
-    | _ => false
-    end)%bool ->
-  (* The rewrite *)
-  uncurry_step
-    (C ⟦ Ffun f ft (k :: fv) (Efun [Ffun g gt gv ge] (Eapp k' kt [g'])) :: fds ⟧)
-    (C ⟦ Put (
-           let '(b, aenv, lm, s, cdata) := ms in
-           (* Set flag to indicate that a rewrite was performed (used to iterate to fixed point) *)
-           let b := true in
-           (* Mark g as uncurried *)
-           let lm := M.set ![g] true lm in
-           (* Update inlining heuristic so inliner knows to inline fully saturated calls to f *)
-           let s := (max (fst s) fp_numargs, (M.set ![f] 1 (M.set ![g] 2 (snd s)))) in
-           (* Hack: update cdata to agree with fresh names generated above *)
-           let cdata :=
-             set_name ![f] ![f1] "_uncurried"
-             (set_names_lst ![fv] ![fv1] ""
-             (set_names_lst ![gv] ![gv1] "" cdata))
-           in
-           (b, aenv, lm, s, cdata) : S_misc)
-         (* Rewrite f as a wrapper around the uncurried f1 and recur on fds *)
-         (Ffun f ft (k :: fv1) (Efun [Ffun g gt gv1 (Eapp f1 ft1 (gv1 ++ fv1))] (Eapp k kt [g]))
-          :: Ffun f1 ft1 (gv ++ fv) ge :: Rec fds) ⟧)
-(* Uncurrying for ANF *)
-| uncurry_anf :
-  forall (C : frames_t exp_univ_list_fundef exp_univ_exp)
-    (f f1 : var) (ft ft1 : fun_tag) (fv fv1 : list var)
-    (g g' : var) (gt : fun_tag) (gv gv1 : list var) (ge : exp) (fds : list fundef)
-    (lhs rhs : list fundef) (s : Ensemble cps.var) (next_x : cps.var)
-    (fp_numargs : nat) (ms : S_misc),
-  (* Non-linear LHS constraints *)
-  g = g' /\
-  (* Guards: *)
-  (* (1) g can't be recursive *)
-  ~ ![g] \in used_vars ![ge] /\
-  (* (2) gv1, fv1, f1 must be fresh and contain no duplicates *)
-  lhs = Ffun f ft fv (Efun [Ffun g gt gv ge] (Ehalt g')) :: fds /\
-  rhs = Ffun f ft fv1 (Efun [Ffun g gt gv1 (Eapp f1 ft1 (gv1 ++ fv1))] (Ehalt g))
-        :: Ffun f1 ft1 (gv ++ fv) ge :: fds /\
-  s = used_vars (exp_of_proto (C ⟦ lhs ⟧)) /\
-  fresh_copies s gv1 /\ length gv1 = length gv /\
-  fresh_copies (s :|: FromList ![gv1]) fv1 /\ length fv1 = length fv /\
-  ~ ![f1] \in (s :|: FromList ![gv1] :|: FromList ![fv1]) /\
-  (* (3) next_x must be a fresh variable *)
-  fresher_than next_x (s :|: FromList ![gv1] :|: FromList ![fv1] :|: [set ![f1]]) /\
-  (* (4) misc. let bindings (needed for computation of new ms) *)
-  fp_numargs = length fv + length gv /\ ms = ms ->
-  (* 'Irrelevant' guard *)
-  When (fun (is_cps : R_misc) (s : S_misc) =>
-    negb is_cps &&
-    let '(b, aenv, lm, s, cdata) := s in
-    (* g must not have been already uncurried by an earlier pass *)
-    negb match M.get ![g] lm with
-    | Some true => true
-    | _ => false
-    end)%bool ->
-  (* The rewrite *)
-  uncurry_step
-    (C ⟦ Ffun f ft fv (Efun [Ffun g gt gv ge] (Ehalt g')) :: fds ⟧)
-    (C ⟦ Put (
-           let '(b, aenv, lm, s, cdata) := ms in
-           (* Set flag to indicate that a rewrite was performed (used to iterate to fixed point) *)
-           let b := true in
-           (* Mark g as uncurried *)
-           let lm := M.set ![g] true lm in
-           (* Update inlining heuristic so inliner knows to inline fully saturated calls to f *)
-           let s := (max (fst s) fp_numargs, (M.set ![f] 1 (M.set ![g] 2 (snd s)))) in
-           (* Hack: update cdata to agree with fresh names generated above *)
-           let cdata :=
-             set_name ![f] ![f1] "_uncurried"
-             (set_names_lst ![fv] ![fv1] ""
-             (set_names_lst ![gv] ![gv1] "" cdata))
-           in
-           (b, aenv, lm, s, cdata) : S_misc)
-         (* Rewrite f as a wrapper around the uncurried f1 and recur on fds *)
-         (Ffun f ft fv1 (Efun [Ffun g gt gv1 (Eapp f1 ft1 (gv1 ++ fv1))] (Ehalt g))
-          :: Ffun f1 ft1 (gv ++ fv) ge :: Rec fds) ⟧).
+(** * Auxiliary data used by the rewriter *)
 
-(** * Uncurrying as a recursive function *)
+(* true if in cps mode *)
+Definition R_C : forall {A}, frames_t A exp_univ_exp -> Set := R_plain bool.
+
+(* pair of 
+   1 - max number of arguments 
+   2 - encoding of inlining decision for beta-contraction phase *)
+Definition St : Set := (nat * (cps.PM nat))%type.
+(* 0 -> Do not inline, 1 -> uncurried function, 2 -> continuation of uncurried function *)
+
+(* Maps (arity+1) to the right fun_tag *)
+Definition arity_map : Set := cps.PM fun_tag.
+Definition local_map : Set := cps.PM bool.
+ 
+(* The state for this includes 
+   1 - a boolean for tracking whether or not a reduction happens
+   2 - Map recording the (new) fun_tag associated to each arity
+   3 - local map from var to if function has already been uncurried
+   4 - Map for uncurried functions for a version of inlining *)
+Definition S_misc : Set := bool * arity_map * local_map * St * comp_data.
 
 (* Based on [get_fun_tag] from uncurry.v *)
 Definition get_fun_tag (n : N) (ms : S_misc) : fun_tag * S_misc :=
@@ -187,6 +73,77 @@ Definition get_fun_tag (n : N) (ms : S_misc) : fun_tag * S_misc :=
     end
   end.
 
+Inductive uncurry_step : exp -> exp -> Prop :=
+(* Uncurrying for CPS *)
+| uncurry_cps :
+  forall (C : frames_t exp_univ_list_fundef exp_univ_exp)
+    (f f1 : var) (ft ft1 : fun_tag) (k k' : var) (kt : fun_tag) (fv fv1 : list var)
+    (g g' : var) (gt : fun_tag) (gv gv1 : list var) (ge : exp) (fds : list fundef)
+    (lhs rhs : list fundef) (s : Ensemble cps.var) (next_x : cps.var)
+    fp_numargs (ms ms' : S_misc),
+  (* Non-linear LHS constraints *)
+  k = k' /\
+  g = g' /\
+  (* Guards: *)
+  (* (1) g can't be recursive or invoke k *)
+  ~ ![g] \in used_vars ![ge] /\
+  ~ ![k] \in used_vars ![ge] /\
+  (* (2) gv1, fv1, f1 must be fresh and contain no duplicates *)
+  lhs = Ffun f ft (k :: fv) (Efun [Ffun g gt gv ge] (Eapp k' kt [g'])) :: fds /\
+  rhs = Ffun f ft (k :: fv1) (Efun [Ffun g gt gv1 (Eapp f1 ft1 (gv1 ++ fv1))] (Eapp k kt [g]))
+        :: Ffun f1 ft1 (gv ++ fv) ge :: fds /\
+  s = used_vars (exp_of_proto (C ⟦ lhs ⟧)) /\
+  fresh_copies s gv1 /\ length gv1 = length gv /\
+  fresh_copies (s :|: FromList ![gv1]) fv1 /\ length fv1 = length fv /\
+  ~ ![f1] \in (s :|: FromList ![gv1] :|: FromList ![fv1]) /\
+  (* (3) next_x must be a fresh variable *)
+  fresher_than next_x (s :|: FromList ![gv1] :|: FromList ![fv1] :|: [set ![f1]]) /\
+  (* (4) generate fun_tag + update ms *)
+  fp_numargs = length fv + length gv /\
+  (ft1, ms') = get_fun_tag (N.of_nat fp_numargs) ms ->
+  (* The rewrite *)
+  uncurry_step
+    (C ⟦ Ffun f ft (k :: fv) (Efun [Ffun g gt gv ge] (Eapp k' kt [g'])) :: fds ⟧)
+    (C ⟦ (* Rewrite f as a wrapper around the uncurried f1 and recur on fds *)
+         (Ffun f ft (k :: fv1) (Efun [Ffun g gt gv1 (Eapp f1 ft1 (gv1 ++ fv1))] (Eapp k kt [g]))
+          :: Ffun f1 ft1 (gv ++ fv) ge :: Rec fds) ⟧)
+(* Uncurrying for ANF *)
+| uncurry_anf :
+  forall (C : frames_t exp_univ_list_fundef exp_univ_exp)
+    (f f1 : var) (ft ft1 : fun_tag) (fv fv1 : list var)
+    (g g' : var) (gt : fun_tag) (gv gv1 : list var) (ge : exp) (fds : list fundef)
+    (lhs rhs : list fundef) (s : Ensemble cps.var) (next_x : cps.var)
+    fp_numargs (ms ms' : S_misc),
+  (* Non-linear LHS constraints *)
+  g = g' /\
+  (* Guards: *)
+  (* (1) g can't be recursive *)
+  ~ ![g] \in used_vars ![ge] /\
+  (* (2) gv1, fv1, f1 must be fresh and contain no duplicates *)
+  lhs = Ffun f ft fv (Efun [Ffun g gt gv ge] (Ehalt g')) :: fds /\
+  rhs = Ffun f ft fv1 (Efun [Ffun g gt gv1 (Eapp f1 ft1 (gv1 ++ fv1))] (Ehalt g))
+        :: Ffun f1 ft1 (gv ++ fv) ge :: fds /\
+  s = used_vars (exp_of_proto (C ⟦ lhs ⟧)) /\
+  fresh_copies s gv1 /\ length gv1 = length gv /\
+  fresh_copies (s :|: FromList ![gv1]) fv1 /\ length fv1 = length fv /\
+  ~ ![f1] \in (s :|: FromList ![gv1] :|: FromList ![fv1]) /\
+  (* (3) next_x must be a fresh variable *)
+  fresher_than next_x (s :|: FromList ![gv1] :|: FromList ![fv1] :|: [set ![f1]]) /\
+  (* (4) generate fun_tag + update ms *)
+  fp_numargs = length fv + length gv /\
+  (ft1, ms') = get_fun_tag (N.of_nat fp_numargs) ms ->
+  (* The rewrite *)
+  uncurry_step
+    (C ⟦ Ffun f ft fv (Efun [Ffun g gt gv ge] (Ehalt g')) :: fds ⟧)
+    (C ⟦ (* Rewrite f as a wrapper around the uncurried f1 and recur on fds *)
+         (Ffun f ft fv1 (Efun [Ffun g gt gv1 (Eapp f1 ft1 (gv1 ++ fv1))] (Ehalt g))
+          :: Ffun f1 ft1 (gv ++ fv) ge :: Rec fds) ⟧).
+
+Definition S : forall {A}, frames_t A exp_univ_exp -> univD A -> Set :=
+  S_prod (S_plain (@S_misc)) (@S_fresh).
+
+(** * Uncurrying as a recursive function *)
+
 Set Printing Universes.
 
 Lemma bool_true_false b : b = false -> b <> true. Proof. now destruct b. Qed.
@@ -194,41 +151,50 @@ Lemma bool_true_false b : b = false -> b <> true. Proof. now destruct b. Qed.
 Local Ltac clearpose H x e :=
   pose (x := e); assert (H : x = e) by (subst x; reflexivity); clearbody x.
 
+Definition metadata_update (f g f1 : var) fp_numargs (fv gv fv1 gv1 : list var) (ms : S_misc) : S_misc :=
+  let '(b, aenv, lm, s, cdata) := ms in
+  (* Set flag to indicate that a rewrite was performed (used to iterate to fixed point) *)
+  let b := true in
+  (* Mark g as uncurried *)
+  let lm := M.set ![g] true lm in
+  (* Update inlining heuristic so inliner knows to inline fully saturated calls to f *)
+  let s := (max (fst s) fp_numargs, (M.set ![f] 1 (M.set ![g] 2 (snd s)))) in
+  (* Hack: update cdata to agree with fresh names generated above *)
+  let cdata :=
+    set_name ![f] ![f1] "_uncurried"
+    (set_names_lst ![fv] ![fv1] ""
+    (set_names_lst ![gv] ![gv1] "" cdata))
+  in
+  (b, aenv, lm, s, cdata).
+
 Definition rw_uncurry :
-  rewriter exp_univ_exp uncurry_step R_misc S_misc
-    (@trivial_delay_t) (@trivial_R_C) (@trivial_R_e) (@S_fresh).
+  rewriter exp_univ_exp uncurry_step (@trivial_delay_t) (@R_C) (@S).
 Proof.
-  mk_rw;
-    (* This particular rewriter's delayed computation is just the identity function,
-       so ConstrDelay and EditDelay are easy *)
-    try lazymatch goal with
-    | |- ConstrDelay _ -> _ =>
-      clear; simpl; intros; lazymatch goal with H : forall _, _ |- _ => eapply H; try reflexivity; eauto end
-    | |- EditDelay _ -> _ =>
-      clear; simpl; intros; lazymatch goal with H : forall _, _ |- _ => eapply H; try reflexivity; eauto end
-    end.
+  mk_rw; mk_easy_delay.
   (* Obligation 1: uncurry_cps side conditions *)
   - intros. rename X into success, H0 into failure.
     (* Check nonlinearities *)
     destruct k as [k], k' as [k'], g as [g], g' as [g'].
-    destruct (eq_var k k') eqn:Hkk'; [|exact failure].
-    destruct (eq_var g g') eqn:Hgg'; [|exact failure].
+    destruct (eq_var k k') eqn:Hkk'; [|cond_failure].
+    destruct (eq_var g g') eqn:Hgg'; [|cond_failure].
     rewrite Pos.eqb_eq in Hkk', Hgg'.
-    (* Check whether g has already been uncurried before *)
+    (* Unpack parameter and state *)
+    rename r_C into mr; unfold R_C, R_plain in mr.
+    destruct s as [ms [next_x Hnext_x]] eqn:Hs.
     destruct ms as [[[[b aenv] lm] heuristic] cdata] eqn:Hms.
+    (* Check whether g has already been uncurried before *)
     destruct (mr && negb (match M.get g lm with Some true => true | _ => false end))%bool
-      as [|] eqn:Huncurried; [|exact failure].
+      as [|] eqn:Huncurried; [|cond_failure].
     (* Check that {g, k} ∩ vars(ge) = ∅ *)
-    destruct (occurs_in_exp g ![ge]) eqn:Hocc_g; [exact failure|]. (* TODO: avoid the conversion *)
-    destruct (occurs_in_exp k ![ge]) eqn:Hocc_k; [exact failure|]. (* TODO: avoid the conversion *)
+    destruct (occurs_in_exp g ![ge]) eqn:Hocc_g; [cond_failure|]. (* TODO: avoid the conversion *)
+    destruct (occurs_in_exp k ![ge]) eqn:Hocc_k; [cond_failure|]. (* TODO: avoid the conversion *)
     apply bool_true_false in Hocc_g; apply bool_true_false in Hocc_k.
     rewrite occurs_in_exp_iff_used_vars in Hocc_g, Hocc_k.
     (* Generate ft1 + new misc state ms *)
     pose (fp_numargs := length fv + length gv).
-    destruct (get_fun_tag (N.of_nat fp_numargs) ms) as [ft1 ms'] eqn:Hget_ft.
-    specialize success with (ft1 := ft1) (ms := ms') (fp_numargs := fp_numargs).
+    specialize success with (ms := ms) (fp_numargs := fp_numargs).
+    destruct (get_fun_tag (BinNatDef.N.of_nat fp_numargs) ms) as [ft1 ms'].
     (* Generate f1, fv1, gv1, next_x *)
-    destruct s as [next_x Hnext_x].
     clearpose Hxgv1 xgv1 (gensyms next_x gv); destruct xgv1 as [next_x0 gv1].
     clearpose Hxfv1 xfv1 (gensyms next_x0 fv); destruct xfv1 as [next_x1 fv1].
     clearpose Hf1 f1 next_x1.
@@ -245,22 +211,24 @@ Proof.
   - intros. rename X0 into success, H0 into failure.
     (* Check nonlinearities *)
     destruct g as [g], g' as [g'].
-    destruct (eq_var g g') eqn:Hgg'; [|exact failure].
+    destruct (eq_var g g') eqn:Hgg'; [|cond_failure].
     rewrite Pos.eqb_eq in Hgg'.
-    (* Check whether g has already been uncurried before *)
+    (* Unpack parameter and state *)
+    rename r_C into mr; unfold R_C, R_plain in mr.
+    destruct s as [ms [next_x Hnext_x]] eqn:Hs.
     destruct ms as [[[[b aenv] lm] heuristic] cdata] eqn:Hms.
+    (* Check whether g has already been uncurried before *)
     destruct (negb mr && negb (match M.get g lm with Some true => true | _ => false end))%bool
-      as [|] eqn:Huncurried; [|exact failure].
+      as [|] eqn:Huncurried; [|cond_failure].
     (* Check that {g, k} ∩ vars(ge) = ∅ *)
-    destruct (occurs_in_exp g ![ge]) eqn:Hocc_g; [exact failure|]. (* TODO: avoid the conversion *)
+    destruct (occurs_in_exp g ![ge]) eqn:Hocc_g; [cond_failure|]. (* TODO: avoid the conversion *)
     apply bool_true_false in Hocc_g.
     rewrite occurs_in_exp_iff_used_vars in Hocc_g.
     (* Generate ft1 + new misc state ms *)
     pose (fp_numargs := length fv + length gv).
-    destruct (get_fun_tag (N.of_nat fp_numargs) ms) as [ft1 ms'] eqn:Hget_ft.
-    specialize success with (ft1 := ft1) (ms := ms') (fp_numargs := fp_numargs).
+    specialize success with (ms := ms) (fp_numargs := fp_numargs).
+    destruct (get_fun_tag (BinNatDef.N.of_nat fp_numargs) ms) as [ft1 ms'].
     (* Generate f1, fv1, gv1, next_x *)
-    destruct s as [next_x Hnext_x].
     clearpose Hxgv1 xgv1 (gensyms next_x gv); destruct xgv1 as [next_x0 gv1].
     clearpose Hxfv1 xfv1 (gensyms next_x0 fv); destruct xfv1 as [next_x1 fv1].
     clearpose Hf1 f1 next_x1.
@@ -273,70 +241,67 @@ Proof.
     + apply fresher_than_not_In; subst f1; exact Hfresh_fv.
     + apply fresher_than_Union; [|subst; simpl; intros y Hy; inversion Hy; lia].
       eapply fresher_than_monotonic; eauto; lia.
-  (* Obligation 3: explain how to maintain fresh name invariant across uncurry_cps *)
-  - clear; unfold Put, Rec; intros.
-    (* Env is easy, because the uncurryer doesn't need it *)
-    split; [exact tt|].
-    (* For state, need create a fresh variable. Thankfully, we have one: next_x *)
-    exists next_x; repeat match goal with H : _ /\ _ |- _ => destruct H end.
-    eapply fresher_than_antimon; [|eassumption].
-    rewrite used_iso, isoABA, used_app.
-    subst s lhs. change (exp_of_proto ?A) with ![A].
-    rewrite used_iso, isoABA, used_app.
-    unfold used; simpl; unbox_newtypes.
-    do 10 normalize_used_vars'; repeat normalize_sets.
-    repeat rewrite strip_vars_app; repeat normalize_sets.
-    intros arbitrary; repeat rewrite In_or_Iff_Union; tauto.
-  (* Obligation 4: explain how to maintain fresh name invariant across uncurry_anf *)
-  - clear; unfold Put, Rec; intros.
-    (* Env is easy, because the uncurryer doesn't need it *)
-    split; [exact tt|].
-    (* For state, need create a fresh variable. Thankfully, we have one: next_x *)
-    exists next_x; repeat match goal with H : _ /\ _ |- _ => destruct H end.
-    eapply fresher_than_antimon; [|eassumption].
-    rewrite used_iso, isoABA, used_app.
-    subst s lhs. change (exp_of_proto ?A) with ![A].
-    rewrite used_iso, isoABA, used_app.
-    unfold used; simpl; unbox_newtypes.
-    do 10 normalize_used_vars'; repeat normalize_sets.
-    repeat rewrite strip_vars_app; repeat normalize_sets.
-    intros arbitrary; repeat rewrite In_or_Iff_Union; tauto.
+  (* Obligation 3: explain how to update state across uncurry_cps *)
+  - clear; unfold Rec; intros; split; [assumption|].
+    (* There are two parts: update various pieces of metadata and show that next_x is still fresh *)
+    split.
+    + exact (metadata_update f g f1 fp_numargs fv gv fv1 gv1 ms').
+    + exists next_x; repeat match goal with H : _ /\ _ |- _ => destruct H end.
+      eapply fresher_than_antimon; [|eassumption].
+      rewrite used_iso, isoABA, used_app.
+      subst s lhs. change (exp_of_proto ?A) with ![A].
+      rewrite used_iso, isoABA, used_app.
+      unfold used; simpl; unbox_newtypes.
+      do 10 normalize_used_vars'; repeat normalize_sets.
+      rewrite !strip_vars_app; repeat normalize_sets.
+      intros arbitrary; rewrite !In_or_Iff_Union; tauto.
+  (* Obligation 4: update state across uncurry_anf.
+     The proof script ends up being identical to obligation 3 *)
+  - clear; unfold Rec; intros; split; [assumption|]; split.
+    + exact (metadata_update f g f1 fp_numargs fv gv fv1 gv1 ms').
+    + exists next_x; repeat match goal with H : _ /\ _ |- _ => destruct H end.
+      eapply fresher_than_antimon; [|eassumption].
+      rewrite used_iso, isoABA, used_app.
+      subst s lhs. change (exp_of_proto ?A) with ![A].
+      rewrite used_iso, isoABA, used_app.
+      unfold used; simpl; unbox_newtypes.
+      do 10 normalize_used_vars'; repeat normalize_sets.
+      rewrite !strip_vars_app; repeat normalize_sets.
+      intros arbitrary; rewrite !In_or_Iff_Union; tauto.
 Defined.
 
 (* Check rw_uncurry. *)
 (* Recursive Extraction rw_uncurry. *)
 
 Lemma uncurry_one (cps : bool) (ms : S_misc) (e : exp) (s : S_fresh <[]> e)
-  : option (result exp_univ_exp uncurry_step S_misc (@S_fresh) <[]> e).
+  : option (result exp_univ_exp uncurry_step (@S) <[]> e).
 Proof.
-  pose (res := run_rewriter' rw_uncurry cps ms e tt tt s); destruct res eqn:Hres.
-  exact (let '(b, _, _, _, _) := resSMisc in if b then Some res else None).
+  pose (res := run_rewriter' rw_uncurry e cps (ms, s)); destruct res eqn:Hres.
+  exact (let '((b, _, _, _, _), _) := resState in if b then Some res else None).
 Defined.
 
 Fixpoint uncurry_fuel (cps : bool) (n : nat) (ms : S_misc) (e : exp) (s : S_fresh <[]> e) {struct n}
-  : result exp_univ_exp uncurry_step S_misc (@S_fresh) <[]> e.
+  : result exp_univ_exp uncurry_step (@S) <[]> e.
 Proof.
   destruct n as [|n].
-  - unshelve econstructor; [exact e|auto|auto|apply Relation_Operators.rt_refl].
+  - unshelve econstructor; [exact e|exact (ms, s)|do 2 constructor].
   - pose (res := uncurry_one cps ms e s).
     refine (match res with Some res' => _ | None => _ end).
     + destruct res'.
-      destruct resSMisc as [[[[_ aenv] lm] st] cdata].
+      destruct resState as [[[[[_ aenv] lm] st] cdata] resState].
       destruct (uncurry_fuel cps n (false, aenv, lm, st, cdata) resTree resState)
-        as [resTree' resState' resSMisc' resProof'].
-      unshelve econstructor; [exact resTree'|auto|auto|].
+        as [resTree' resState' resProof'].
+      unshelve econstructor; [exact resTree'|auto|].
       eapply Relation_Operators.rt_trans; eauto.
-    + unshelve econstructor; [exact e|auto|auto|apply Relation_Operators.rt_refl].
+    + unshelve econstructor; [exact e|exact (ms, s)|apply Relation_Operators.rt_refl].
 Defined.
 
 Definition uncurry_top (cps : bool) (n : nat) (cdata : comp_data) (e : exp) : exp * M.t nat * comp_data.
 Proof.
-  refine (let '{| resTree := e'; resSMisc := ms |} := uncurry_fuel cps n _ e _ in _).
+  refine (
+    let '{| resTree := e'; resState := (ms, _) |} := uncurry_fuel cps n _ e (initial_fresh e) in
+    _).
   - exact (false, M.empty _, M.empty _, (0%nat, (M.empty _)), cdata).
-  - exists (1 + max_var ![e] 1)%positive.
-    change (![ <[]> ⟦ ?e ⟧ ]) with ![e]; unfold fresher_than.
-    intros y Hy; enough (y <= max_var ![e] 1)%positive by lia.
-    destruct Hy; [now apply bound_var_leq_max_var|now apply occurs_free_leq_max_var].
   - destruct ms as [[[[_ _] _] [_ st]] cdata'].
     exact (e', st, cdata').
 Defined.
